core/EvalExpr.v
@@ -1,0 +1,164 @@
+Require Import Coq.Strings.String.
+Require Import Poulet4.Typed.
+Require Import Poulet4.Syntax.
+Require Import Poulet4.Semantics.
+Require Import ProD3.core.Coqlib.
+Require Import ProD3.core.Hoare.
+Require Import ProD3.core.AssertionLang.
+Require Import Coq.ZArith.BinInt.
+Require Import Hammer.Tactics.Tactics.
+Require Import Hammer.Plugin.Hammer.
+
+Section EvalExpr.
+
+Context {tags_t: Type} {tags_t_inhabitant : Inhabitant tags_t}.
+Notation Val := (@ValueBase bool).
+Notation Sval := (@ValueBase (option bool)).
+Notation Lval := (ValueLvalue).
+
+Notation ident := (string).
+Notation path := (list ident).
+Notation P4Int := (P4Int.t tags_t).
+Notation P4String := (P4String.t tags_t).
+Notation P4Type := (@P4Type tags_t).
+Notation Expression := (@Expression tags_t).
+
+Context `{@Target tags_t Expression}.
+
+(* Convert Sval to Val only when all bits are known. *)
+Axiom eval_sval_to_val : Sval -> option Val.
+
+(* Convert Sval to Val, convert unknown bits to false. *)
+Axiom force_sval_to_val : Sval -> Val.
+
+(* Convert Val to Sval, but convert all bits to unknown. *)
+Axiom val_to_liberal_sval : Val -> Sval.
+
+Definition build_abs_unary_op (actual_unary_op : Val -> option Val) : Sval -> Sval :=
+  fun sv =>
+    match eval_sval_to_val sv with
+    | Some v =>
+        eval_val_to_sval (force ValBaseNull (actual_unary_op v))
+    | _ =>
+        let v := force_sval_to_val sv in
+        val_to_liberal_sval (force ValBaseNull (actual_unary_op v))
+    end.
+
+(* "Not" under abstract interpretation. *)
+Definition abs_not : Sval -> Sval :=
+  build_abs_unary_op (Ops.eval_unary_op Not).
+
+Definition build_abs_binary_op (actual_binany_op : Val -> Val -> option Val) : Sval -> Sval -> Sval :=
+  fun sv1 sv2 =>
+    match eval_sval_to_val sv1, eval_sval_to_val sv2 with
+    | Some v1, Some v2 =>
+        eval_val_to_sval (force ValBaseNull (actual_binany_op v1 v2))
+    | _, _ =>
+        let v1 := force_sval_to_val sv1 in
+        let v2 := force_sval_to_val sv2 in
+        val_to_liberal_sval (force ValBaseNull (actual_binany_op v1 v2))
+    end.
+
+(* Plus under abstract interpretation. *)
+Definition abs_plus : Sval -> Sval -> Sval :=
+  build_abs_binary_op (Ops.eval_binary_op Plus).
+
+Definition abs_minus : Sval -> Sval -> Sval :=
+  build_abs_binary_op (Ops.eval_binary_op Minus).
+
+Axiom abs_plus_bit : forall w i1 i2,
+  abs_plus
+    (ValBaseBit (P4Arith.to_loptbool w i1))
+    (ValBaseBit (P4Arith.to_loptbool w i2))
+  = (ValBaseBit (P4Arith.to_loptbool w (i1 + i2))).
+
+Fixpoint eval_read (a : mem_assertion) (p : path) : option Sval :=
+  match a with
+  | (p', v) :: tl =>
+      if path_eqb p p' then Some v else eval_read tl p
+  | [] => None
+  end.
+
+Fixpoint eval_expr (ge : genv) (p : path) (a : mem_assertion) (expr : Expression) : option Sval :=
+  match expr with
+  | MkExpression _ expr _ dir =>
+      match expr with
+      | ExpInt i => Some (eval_p4int_sval i)
+      | ExpName _ loc =>
+          if is_directional dir then
+            match loc with
+            | LInstance p => eval_read a p
+            | _ => None
+            end
+          else
+            option_map eval_val_to_sval (loc_to_val_const ge p loc)
+      | ExpUnaryOp op arg =>
+          match eval_expr ge p a arg with
+          | Some argv => Some (build_abs_unary_op (Ops.eval_unary_op op) argv)
+          | None => None
+          end
+      | ExpBinaryOp op (larg, rarg) =>
+          match eval_expr ge p a larg, eval_expr ge p a rarg with
+          | Some largv, Some rargv => Some (build_abs_binary_op (Ops.eval_binary_op op) largv rargv)
+          | _, _ => None
+          end
+      (* | ExpCast newtyp arg =>
+          match eval_expr_gen hook arg, get_real_type newtyp with
+          | Some argv, Some real_typ => Ops.eval_cast real_typ argv
+          | _, _ => None
+          end *)
+      | ExpExpressionMember expr name =>
+          match eval_expr ge p a expr with
+          | Some sv =>
+              Some (get (P4String.str name) sv)
+          | None => None
+          end
+      | _ => None
+      end
+  end.
+
+Lemma get_member_sound : forall sv f sv',
+  match sv with ValBaseStruct _ | ValBaseHeader _ _ => true | _ => false end ->
+  get_member sv f sv' ->
+  get f sv = sv'.
+Proof.
+  intros.
+  destruct sv; try solve [inv H0]; inv H1.
+  - unfold get. rewrite H3. auto.
+  - unfold get. rewrite H6. auto.
+Qed.
+
+Lemma eval_expr_member_sound : forall ge p a tags expr typ dir name sv,
+  match sv with ValBaseStruct _ | ValBaseHeader _ _ => true | _ => false end ->
+  hoare_expr ge p a expr sv ->
+  hoare_expr ge p a (MkExpression tags (ExpExpressionMember expr name) typ dir) (get (P4String.str name) sv).
+Proof.
+  unfold hoare_expr.
+  intros.
+  inv H3.
+  assert (sval_refine sv sv0) by (eapply H1; eauto).
+  apply get_member_sound in H13. 2 : {
+    inv H3; try solve [inv H0]; auto.
+  }
+  rewrite <- H13.
+  admit.
+    (* sval_refine sv sv0 ->
+      sval_refine (get (P4String.str name) sv) (get (P4String.str name) sv0) *)
+Admitted.
+
+Lemma eval_expr_sound' : forall ge p a expr sv,
+  eval_expr ge p a expr = Some sv ->
+  forall st, (mem_denote a) (fst st) ->
+  forall sv', exec_expr ge read_ndetbit p st expr sv' ->
+    sval_refine sv sv'.
+Admitted.
+
+Lemma eval_expr_sound : forall ge p a expr sv,
+  eval_expr ge p a expr = Some sv ->
+  hoare_expr ge p (fun st => mem_denote a (fst st)) expr sv.
+Proof.
+  unfold hoare_expr; intros.
+  eapply eval_expr_sound'; eauto.
+Qed.
+
+End EvalExpr.
