examples/expr/ExprTests.v
@@ -6,17 +6,18 @@ Require Import Poulet4.Semantics.
 Require Import ProD3.core.Coqlib.
 Require Import ProD3.core.Hoare.
 Require Import ProD3.core.AssertionLang.
+Require Import ProD3.core.EvalExpr.
 Require Import Hammer.Tactics.Tactics.
 Require Import Hammer.Plugin.Hammer.
 Import Poulet4.Semantics.
 Open Scope string_scope.
 
 Section ExprTests.
-
 Context `{@Target Info (@Expression Info)}.
 Notation Val := (@ValueBase bool).
 Notation Sval := (@ValueBase (option bool)).
 Notation Lval := (ValueLvalue).
+Notation Expression := (@Expression Info).
 
 Notation ident := (string).
 Notation path := (list ident).
@@ -135,8 +136,6 @@ Definition mem_pre2 : mem_assertion :=
 Definition pre2 : assertion := fun '(m, es) =>
   mem_denote mem_pre2 m.
 
-Axiom get : ident -> Sval -> Sval.
-
 Axiom target2 :
   get "x" a = ValBaseBit (P4Arith.to_loptbool 8%N xi) ->
   get "y" a = ValBaseBit (P4Arith.to_loptbool 8%N yi) ->
@@ -145,54 +144,7 @@ Axiom target2 :
 (* So I think we should build a function that eval to (option Sval),
   but only gives None when used variables are not found in the mem_assertion. *)
 
-(* Convert Sval to Val only when all bits are known. *)
-Axiom eval_sval_to_val : Sval -> option Val.
-
-(* Convert Sval to Val, convert unknown bits to false. *)
-Axiom force_sval_to_val : Sval -> Val.
-
-(* Convert Val to Sval, but convert all bits to unknown. *)
-Axiom val_to_liberal_sval : Val -> Sval.
-
-Definition build_abs_unary_op (actual_unary_op : Val -> option Val) : Sval -> Sval :=
-  fun sv =>
-    match eval_sval_to_val sv with
-    | Some v =>
-        eval_val_to_sval (force ValBaseNull (actual_unary_op v))
-    | _ =>
-        let v := force_sval_to_val sv in
-        val_to_liberal_sval (force ValBaseNull (actual_unary_op v))
-    end.
-
-(* "Not" under abstract interpretation. *)
-Definition abs_not : Sval -> Sval :=
-  build_abs_unary_op (Ops.Ops.eval_unary_op Not).
-
-Definition build_abs_binary_op (actual_binany_op : Val -> Val -> option Val) : Sval -> Sval -> Sval :=
-  fun sv1 sv2 =>
-    match eval_sval_to_val sv1, eval_sval_to_val sv2 with
-    | Some v1, Some v2 =>
-        eval_val_to_sval (force ValBaseNull (actual_binany_op v1 v2))
-    | _, _ =>
-        let v1 := force_sval_to_val sv1 in
-        let v2 := force_sval_to_val sv2 in
-        val_to_liberal_sval (force ValBaseNull (actual_binany_op v1 v2))
-    end.
-
-(* Plus under abstract interpretation. *)
-Definition abs_plus : Sval -> Sval -> Sval :=
-  build_abs_binary_op (Ops.Ops.eval_binary_op Plus).
-
-Definition abs_minus : Sval -> Sval -> Sval :=
-  build_abs_binary_op (Ops.Ops.eval_binary_op Minus).
-
-Axiom abs_plus_bit : forall w i1 i2,
-  abs_plus
-    (ValBaseBit (P4Arith.to_loptbool w i1))
-    (ValBaseBit (P4Arith.to_loptbool w i2))
-  = (ValBaseBit (P4Arith.to_loptbool w (i1 + i2))).
 
 
-
-
+Eval simpl in (eval_expr ge p mem_pre1 expr1).
 
